F closed and a value, compat lemma cast

theories/backtranslation/cast_help/between.v
@@ -13,11 +13,11 @@ Proof.
   by simpl.
 Qed.
 
-Definition between_TSum (c1 c2 : expr) : expr :=
-  Lam (Case (Var 0) (InjL ((rename (+2) c1) (Var 0))) (InjR ((rename (+2) c2) (Var 0)))).
+Definition between_TSum (c1 c2 : expr) : val :=
+  LamV (Case (Var 0) (InjL ((rename (+2) c1) (Var 0))) (InjR ((rename (+2) c2) (Var 0)))).
 
 Lemma between_TSum_subst_rewrite σ f1 f2 :
-  (between_TSum f1 f2).[σ] =
+  (# (between_TSum f1 f2)).[σ] =
   between_TSum f1.[σ] f2.[σ].
 Proof.
   rewrite /between_TSum.
@@ -37,11 +37,11 @@ Proof.
   apply up_type_two. apply d2. by apply Var_typed.
 Qed.
 
-Definition between_TProd (f1 f2 : expr) : expr :=
-  Lam (Pair (rename (+1) f1 (Fst (Var 0))) (rename (+1) f2 (Snd (Var 0)))).
+Definition between_TProd (f1 f2 : expr) : val :=
+  LamV (Pair (rename (+1) f1 (Fst (Var 0))) (rename (+1) f2 (Snd (Var 0)))).
 
 Lemma between_TProd_subst_rewrite σ f1 f2 :
-  (between_TProd f1 f2).[σ] =
+  (# (between_TProd f1 f2)).[σ] =
   between_TProd f1.[σ] f2.[σ].
 Proof.
   rewrite /between_TProd.
@@ -59,15 +59,15 @@ Proof.
   apply up_type_one. apply d2. econstructor. by apply Var_typed.
 Qed.
 
-Definition between_TArrow (ca cr : expr) : expr :=
-  Lam (*f*)
+Definition between_TArrow (ca cr : expr) : val :=
+  LamV (*f*)
     (Lam (*a*) (
          rename (+2) cr (((Var 1)(*f*)) (rename (+2) ca (Var 0(*a*))))
        )
     ).
 
 Lemma between_TArrow_subst_rewrite σ ca cr :
-  (between_TArrow ca cr).[σ] =
+  (# (between_TArrow ca cr)).[σ] =
   between_TArrow ca.[σ] cr.[σ].
 Proof.
   rewrite /between_TArrow.
@@ -85,65 +85,7 @@ Proof.
     by apply Var_typed.
 Qed.
 
-Definition between_TRec (f : expr) : expr :=
-  Lam (* x : μ. τi *) (
-      Fix (
-          Lam (* g : μ.τi → μ.τf *) (
-              Lam (* r : μ.τi *) (
-                  Fold (rename (+1) (f.[upn 1 (ren (+ 1))])(* : τi.[μ.τi/] → τf.[μ.τf]*) (Unfold (Var 0)))
-                )
-            )
-        ) (Var 0)
-    ).
-
-Lemma between_TRec_typed Γ (τi τf : type) (Pi : Is_Closed (TRec τi)) (Pf : Is_Closed (TRec τf)) (f : expr)
-      (d : ((TArrow (TRec τi) (TRec τf)):: Γ) ⊢ₛ f : (TArrow (τi.[TRec τi/]) τf.[TRec τf/])) :
-  Γ ⊢ₛ between_TRec f : (TArrow (stlc_mu.typing.TRec τi) (stlc_mu.typing.TRec τf))%type.
-Proof.
-  apply Lam_typed.
-  apply App_typed with (τ1 := TRec τi).
-  (* apply App_typed with (τ1 := ((TRec τi → TRec τf) → (TRec τi → TRec τf))). *)
-  eapply App_typed.
-  apply Fix_typed; auto.
-    (* by intro τ; simpl; rewrite -(Pi τ); rewrite -(Pf τ); by simpl. *)
-  apply Lam_typed.
-  apply Lam_typed.
-  apply Fold_typed.
-  apply App_typed with (τ1 := τi.[(TRec τi)/]).
-  apply up_type_one.
-  rewrite rewrite_for_context_weakening in d.
-  rewrite (rewrite_for_context_weakening Γ).
-  rewrite rewrite_for_context_weakening.
-  apply context_gen_weakening.
-  apply d.
-  apply Unfold_typed.
-  by apply Var_typed.
-  by apply Var_typed.
-Qed.
-
-Definition between_TRec' (f : expr) : expr :=
-  Lam (* x : μ. τi *) (
-      Fix'' (
-          Lam (* g : μ.τi → μ.τf *) (
-              Lam (* r : μ.τi *) (
-                  Fold (rename (+1) (f.[upn 1 (ren (+ 1))])(* : τi.[μ.τi/] → τf.[μ.τf]*) (Unfold (Var 0)))
-                )
-            )
-        ) (Var 0)
-    ).
-
-Lemma between_TRec'_subst_rewrite σ f :
-  (between_TRec' f).[σ] =
-  between_TRec' f.[up σ].
-Proof.
-  rewrite /between_TRec'.
-  rewrite subst_lam.
-  rewrite subst_app.
-  rewrite Fix''_subs_rewrite.
-  by asimpl.
-Qed.
-
-Definition between_TRecV' (f : expr) : val :=
+Definition between_TRec (f : expr) : val :=
   LamV (* x : μ. τi *) (
       Fix'' (
           Lam (* g : μ.τi → μ.τf *) (
@@ -154,14 +96,27 @@ Definition between_TRecV' (f : expr) : val :=
         ) (Var 0)
     ).
 
-Lemma between_TRec'_to_value f : between_TRec' f = stlc_mu.lang.of_val (between_TRecV' f).
+Lemma between_TRec_subst_rewrite σ f :
+  (# (between_TRec f)).[σ] =
+  between_TRec f.[up σ].
+Proof.
+  rewrite /between_TRec.
+  rewrite subst_lam.
+  rewrite subst_app.
+  rewrite Fix''_subs_rewrite.
+  by asimpl.
+Qed.
+
+Definition between_TRecV (f : expr) : val := between_TRec f.
+
+Lemma between_TRec_to_value f : stlc_mu.lang.of_val (between_TRec f) = stlc_mu.lang.of_val (between_TRecV f).
 Proof.
   by simpl.
 Qed.
 
-Lemma between_TRec'_typed Γ (τi τf : type) (Pi : Is_Closed (TRec τi)) (Pf : Is_Closed (TRec τf)) (f : expr)
+Lemma between_TRec_typed Γ (τi τf : type) (Pi : Is_Closed (TRec τi)) (Pf : Is_Closed (TRec τf)) (f : expr)
       (d : ((TArrow (TRec τi) (TRec τf)):: Γ) ⊢ₛ f : (TArrow (τi.[TRec τi/]) τf.[TRec τf/])) :
-  Γ ⊢ₛ between_TRec' f : (TArrow (stlc_mu.typing.TRec τi) (stlc_mu.typing.TRec τf))%type.
+  Γ ⊢ₛ between_TRec f : (TArrow (stlc_mu.typing.TRec τi) (stlc_mu.typing.TRec τf))%type.
 Proof.
   apply Lam_typed.
   apply App_typed with (τ1 := TRec τi).
@@ -181,65 +136,3 @@ Proof.
   by apply Var_typed.
   by apply Var_typed.
 Qed.
-
-Definition between_TRec_stepped (f : expr) : expr :=
-  Lam (* x : μ. τi *) (
-      Fix_stepped.[(
-          Lam (* g : μ.τi → μ.τf *) (
-              Lam (* r : μ.τi *) (
-                  Fold (rename (+1) (f.[upn 1 (ren (+ 1))])(* : τi.[μ.τi/] → τf.[μ.τf]*) (Unfold (Var 0)))
-                )
-            )
-        )/] (Var 0)
-    ).
-
-Lemma between_TRec_stepped_typed Γ (τi τf : type) (Pi : Is_Closed (TRec τi)) (Pf : Is_Closed (TRec τf)) (f : expr)
-      (d : ((TArrow (TRec τi) (TRec τf)):: Γ) ⊢ₛ f : (TArrow (τi.[TRec τi/]) τf.[TRec τf/])) :
-  Γ ⊢ₛ between_TRec_stepped f : (TArrow (stlc_mu.typing.TRec τi) (stlc_mu.typing.TRec τf))%type.
-Proof.
-  apply Lam_typed.
-  apply App_typed with (τ1 := TRec τi).
-  apply Fix_stepped_subs_typed; auto.
-    (* by intro τ; simpl; rewrite -(Pi τ); rewrite -(Pf τ); by simpl. *)
-  apply Lam_typed.
-  apply Lam_typed.
-  apply Fold_typed.
-  apply App_typed with (τ1 := τi.[(TRec τi)/]).
-  apply up_type_one.
-  rewrite rewrite_for_context_weakening in d.
-  rewrite (rewrite_for_context_weakening Γ).
-  rewrite rewrite_for_context_weakening.
-  apply context_gen_weakening.
-  apply d.
-  apply Unfold_typed.
-  by apply Var_typed.
-  by apply Var_typed.
-Qed.
-
-(* Lemma between_TRec_subs (f : expr) σ : (between_TRec_stepped f).[σ] = between_TRec_stepped (f.[ids 0 .: σ]). *)
-(* Proof. *)
-(*   rewrite /between_TRec_stepped /Fix_stepped. *)
-(*   asimpl. *)
-(*   auto. *)
-(*   repeat rewrite rename_ren. *)
-(*   simpl. *)
-(*   f_equal. *)
-(*   f_equal. *)
-(*   f_equal. *)
-(*   f_equal. *)
-(*   f_equal. *)
-(*   f_equal. *)
-(*   f_equal. *)
-(*   repeat rewrite subst_comp. repeat rewrite up_lift1. asimpl. *)
-(*   rewrite -fold_ren_cons *)
-
-
-(*   admit. *)
-(*   asimpl. *)
-(*   asimpl. *)
-(*   asimpl. *)
-(*   repeat f_equal. *)
-(*   asimpl.  *)
-(*   rewrite /up. *)
-(*   rewrite -up_comp. *)
-(*   asimpl. *)
