theories/backtranslation/cast_help/general.v
@@ -31,25 +31,18 @@ Fixpoint 𝓕 {A : list (types.type * types.type)} {τi τf : cast_calculus.type
       (𝓕 pCons31)
       (𝓕 pCons24)
   | consTRecTRecExposeCall _ τl τr pμτlμτrnotA pUnfτlUnfτr =>
-    between_TRec'
+    between_TRec
       (𝓕 pUnfτlUnfτr)
   (* | consTRecTRecUseCall _ τl τr i pμτlμtrinA => Lam ((Var (S i)) (Var 0)) *)
   | consTRecTRecUseCall _ τl τr i pμτlμtrinA => Var i
   end.
-
-(* Lemma 𝓕_is_value {A} {τi τf} (pC : A ⊢ τi ~ τf) : is_Some $ to_val (𝓕 pC). *)
-(* Proof. *)
-(*   induction pC; try destruct G; simplify_option_eq; eauto. *)
-(* Qed. *)
-
-(* Definition 𝓕V {A} {τi τf} (pC : A ⊢ τi ~ τf) : val := is_Some_proj (𝓕_is_value pC). *)
 
 From fae_gtlc_mu.stlc_mu Require Export typing lang lib.fix.
 
 Definition pair_to_static_function (p : cast_calculus.types.type * cast_calculus.types.type) : stlc_mu.typing.type :=
   TArrow <<p.1>> <<p.2>>.
 
-Lemma 𝓕_typed (A : list (cast_calculus.types.type * cast_calculus.types.type)) (τi τf : cast_calculus.types.type) (pτiConsτf : A ⊢ τi ~ τf) :
+Lemma 𝓕_typed (A : list (cast_calculus.types.type * cast_calculus.types.type)) (τi τf : cast_calculus.types.type) (pτi : TClosed τi) (pτf : TClosed τf) (pτiConsτf : A ⊢ τi ~ τf) :
   (map pair_to_static_function A) ⊢ₛ (𝓕 pτiConsτf) : (TArrow <<τi>> <<τf>>).
 Proof.
   induction pτiConsτf; simpl.
@@ -57,26 +50,119 @@ Proof.
   - apply embed_typed.
   - apply factorization_up_typed.
     apply IHpτiConsτf.
+    done. admit.
   - apply factorization_down_typed.
     apply IHpτiConsτf.
+    admit. admit.
   - apply identity_typed.
   - apply identity_typed.
   - apply between_TSum_typed.
     apply IHpτiConsτf1.
+    admit. admit.
     apply IHpτiConsτf2.
+    admit. admit.
   - apply between_TProd_typed.
     apply IHpτiConsτf1.
+    admit. admit.
     apply IHpτiConsτf2.
+    admit. admit.
   - apply between_TArrow_typed.
     apply IHpτiConsτf1.
+    admit. admit.
     apply IHpτiConsτf2.
-  - apply between_TRec'_typed.
-    admit.
-    admit.
+    admit. admit.
+  - apply between_TRec_typed.
+    admit. admit.
     rewrite map_cons in IHpτiConsτf.
     repeat rewrite unfolding_backtranslation_commutes in IHpτiConsτf.
     apply IHpτiConsτf.
+    admit. admit.
   - apply Var_typed.
     rewrite list_lookup_fmap.
     by rewrite pμτlμtrinA.
+Admitted.
+
+
+Definition 𝓕c {A} {τi τf} (pC : cons_struct A τi τf) fs : stlc_mu.lang.expr :=
+  (𝓕 pC).[stlc_mu.typing.env_subst fs].
+
+(** 𝓕 pC is a value after substitution *)
+
+Definition 𝓕cV {A} {τi τf} (pC : cons_struct A τi τf) fs (H : length A = length fs) : stlc_mu.lang.val :=
+  match to_val (𝓕c pC fs) with
+  | Some x => x
+  | None => UnitV
+  end.
+
+Lemma 𝓕c_rewrite {A} {τi τf} (pC : cons_struct A τi τf) fs (H : length A = length fs) : 𝓕c pC fs = # (𝓕cV pC fs H).
+Proof.
+  unfold 𝓕cV.
+  destruct pC.
+  - rewrite /𝓕c /𝓕. by rewrite extract_no_subs to_of_val.
+  - rewrite /𝓕c /𝓕. by rewrite embed_no_subs to_of_val.
+  - rewrite /𝓕c /𝓕. rewrite factorization_up_subst_rewrite. fold (𝓕 pC).
+    by rewrite to_of_val.
+  - rewrite /𝓕c /𝓕. rewrite factorization_down_subst_rewrite. fold (𝓕 pC).
+    by rewrite to_of_val.
+  - rewrite /𝓕c /𝓕. by asimpl.
+  - rewrite /𝓕c /𝓕. by asimpl.
+  - rewrite /𝓕c /𝓕. rewrite between_TSum_subst_rewrite.
+    fold (𝓕 pC1).
+    fold (𝓕 pC2).
+    by rewrite to_of_val.
+  - rewrite /𝓕c /𝓕. rewrite between_TProd_subst_rewrite.
+    by rewrite to_of_val.
+  - rewrite /𝓕c /𝓕. rewrite between_TArrow_subst_rewrite.
+    by rewrite to_of_val.
+  - rewrite /𝓕c /𝓕. rewrite between_TRec_subst_rewrite.
+    by rewrite to_of_val.
+  - rewrite /𝓕c /𝓕.
+    assert (Hi : i < length fs). rewrite -H; apply lookup_lt_is_Some; by econstructor.
+    destruct (fs !! i) eqn:Hf.
+    simpl.
+    erewrite env_subst_lookup. by rewrite to_of_val.
+    apply Hf.
+    exfalso.
+    assert (length fs ≤ i). by apply lookup_ge_None_1.
+    lia.
+Qed.
+
+Lemma 𝓕c_closed {A} {τi τf} (pC : cons_struct A τi τf) fs (H : length A = length fs) (Hfsc : Forall VClosed fs) :
+  EClosed (𝓕c pC fs).
+Proof.
+  generalize dependent fs.
+  induction pC; intros fs Hfs Hfsc; rewrite /𝓕c /𝓕.
+  - intro. by repeat rewrite extract_no_subs.
+  - intro. by repeat rewrite embed_no_subs.
+  - fold (𝓕 pC). rewrite factorization_up_subst_rewrite. fold (𝓕c pC fs).
+    intro. asimpl. rewrite embed_no_subs. by repeat rewrite IHpC.
+  - fold (𝓕 pC). rewrite factorization_down_subst_rewrite. fold (𝓕c pC fs).
+    intro. asimpl. rewrite extract_no_subs. by repeat rewrite IHpC.
+  - intro; by asimpl.
+  - intro; by asimpl.
+  - fold (𝓕 pC1). fold (𝓕 pC2).
+    rewrite between_TSum_subst_rewrite.
+    fold (𝓕c pC1 fs). fold (𝓕c pC2 fs).
+    intro; asimpl. repeat rewrite IHpC1; by repeat rewrite IHpC2.
+  - fold (𝓕 pC1). fold (𝓕 pC2).
+    rewrite between_TProd_subst_rewrite.
+    fold (𝓕c pC1 fs). fold (𝓕c pC2 fs).
+    intro; asimpl. repeat rewrite IHpC1; by repeat rewrite IHpC2.
+  - fold (𝓕 pC1). fold (𝓕 pC2).
+    rewrite between_TArrow_subst_rewrite.
+    fold (𝓕c pC1 fs). fold (𝓕c pC2 fs).
+    intro; asimpl. repeat rewrite IHpC1; by repeat rewrite IHpC2.
+  - fold (𝓕 pC).
+    rewrite between_TRec_subst_rewrite.
+    intro.
+    admit.
+  - asimpl.
+    assert (Hi : i < length fs). rewrite -Hfs; apply lookup_lt_is_Some; by econstructor.
+    destruct (fs !! i) eqn:Hf.
+    + rewrite (env_subst_lookup fs _ v).
+      apply ve_closed.
+      eapply (Forall_lookup_1). apply Hfsc. apply Hf. apply Hf.
+    + exfalso.
+      assert (length fs ≤ i). by apply lookup_ge_None_1.
+      lia.
 Admitted.
